Complete bijectivemap

dafny/top-down/bijective_map.dfy
@@ -1,42 +1,118 @@
+include "std-lib/src/Wrappers.dfy"
+
+
 module BijectiveMap {
-    datatype BijectiveMap<T1(!new), T2(!new)> = BijectiveMap(l_to_r:map<T1, T2>, r_to_l:map<T2, T1>) {
+    import opened Wrappers
+
+    datatype BijectiveMap<T1, T2> = BijectiveMap(l_to_r:map<T1, T2>, r_to_l:map<T2, T1>) {
         predicate valid() {
             (forall k:T1 :: k in l_to_r ==>
                 l_to_r[k] in r_to_l && r_to_l[l_to_r[k]] == k)
             && (forall k:T2 :: k in r_to_l ==> 
                 r_to_l[k] in l_to_r && l_to_r[r_to_l[k]] == k)
             // && |l_to_r.Values| == |r_to_l.Values|
-            // && |l_to_r| == |r_to_l| // Dafny should ideally figure this out by itself
+            && |l_to_r| == |r_to_l| // Dafny should ideally figure this out by itself
             // && (forall t1:T1, t2:T2 :: (t1, t2) in l_to_r.Items ==> (t2, t1) in r_to_l.Items)
             // && (forall t1:T1, t2:T2 :: (t2, t1) in r_to_l.Items ==> (t1, t2) in l_to_r.Items)
         }
 
-        lemma lemma_domain_sizes()
-            requires valid()
-            ensures valid()
-            ensures |l_to_r| == |r_to_l|
-        {
-            if (|l_to_r| == 0) {
-                assert(|r_to_l| == 0);
-            } else if |l_to_r| == 1 {
-                assert(exists k:T1 | k in l_to_r :: l_to_r[k] in r_to_l);
-                assert(|r_to_l| == 1);
+        // function method {:opaque} in1(e:T1) : bool
+        //     requires valid()
+        //     ensures in1(e) == (e in l_to_r)
+        // {
+        //     e in l_to_r
+        // }
 
-            }
+        function method in1(e:T1) : bool
+            requires valid()
+            ensures in1(e) == (e in l_to_r)
+        {
+            e in l_to_r
         }
 
-        lemma lemma_domain_range_sizes()
+        function method in2(e:T2) : bool
             requires valid()
-            ensures valid()
-            ensures l_to_r.Values == r_to_l.Keys
-            ensures |l_to_r.Values| == |r_to_l.Keys|
-
-            ensures r_to_l.Values == l_to_r.Keys
-            ensures |r_to_l.Values| == |l_to_r.Keys|
+            ensures in2(e) == (e in r_to_l)
         {
-            lemma_domain_sizes();
-            // assume(|l_to_r| == |r_to_l|);
+            e in r_to_l
         }
+
+        function method get1(e:T1) : T2
+            requires valid()
+            requires in1(e)
+            requires e in l_to_r
+            ensures get1(e) == l_to_r[e]
+        {
+            l_to_r[e]
+        }
+
+        function method insert(e1:T1, e2:T2) : BijectiveMap<T1, T2>
+            requires valid()
+            // requires !in1(e1) && !in2(e2)
+            requires (e1 !in l_to_r && e2 !in r_to_l)
+                     || (e1 in l_to_r && e2 == l_to_r[e1] && e2 in r_to_l && e1 == r_to_l[e2])
+            ensures insert(e1, e2).valid()
+            ensures insert(e1, e2) == BijectiveMap(l_to_r[e1 := e2], r_to_l[e2 := e1])
+            ensures insert(e1, e2).in1(e1)
+            ensures insert(e1, e2).in2(e2)
+        {
+            BijectiveMap(l_to_r[e1 := e2], r_to_l[e2 := e1])
+        }
+
+        function method equal(b:BijectiveMap<T1, T2>) : bool
+            requires valid()
+        {
+            forall e1:T1 :: e1 in l_to_r ==> e1 in b.l_to_r
+            && forall e2:T2 :: e2 in r_to_l ==> e2 in b.r_to_l
+        }
+
+
+        function Values() : set<T2>
+            requires valid() // Needed?
+        {
+            r_to_l.Keys
+        }
+
+        function Keys() : set<T1>
+            requires valid() // Needed?
+        {
+            l_to_r.Keys
+        }
+
+        function Items() : set<(T1, T2)>
+            requires valid() // Needed?
+        {
+            l_to_r.Items
+        }
+
+        // lemma lemma_domain_sizes(b:BijectiveMap<T1, T2>)
+        //     requires b.valid()
+        //     ensures b.valid()
+        //     ensures |b.l_to_r| == |b.r_to_l|
+        // {
+        //     // assert(forall k :: k in l_to_r ==> l_to_r[k] in r_to_l);
+        //     // assert (|l_to_r.Values| == |r_to_l.Keys|);
+        //     // assert (|l_to_r| == |l_to_r.Values|);
+        //     if |b.l_to_r| == 0 {
+        //         assert(|b.l_to_r| == |b.r_to_l|);
+        //     } else {
+        //         var K:T1;
+        //         assume (K in b.l_to_r);
+        //     }
+        // }
+
+        // lemma lemma_domain_range_sizes()
+        //     requires valid()
+        //     ensures valid()
+        //     ensures l_to_r.Values == r_to_l.Keys
+        //     ensures |l_to_r.Values| == |r_to_l.Keys|
+
+        //     ensures r_to_l.Values == l_to_r.Keys
+        //     ensures |r_to_l.Values| == |l_to_r.Keys|
+        // {
+        //     lemma_domain_sizes();
+        //     // assume(|l_to_r| == |r_to_l|);
+        // }
 
         // lemma same_size()
         //     requires valid()
@@ -52,5 +128,16 @@ module BijectiveMap {
         //     assert(|l_to_r| == |r_to_l|);
         //     // assert(valid());
         // }
+    }
+
+    method new_bijective_map<T1, T2> () returns (b:BijectiveMap<T1, T2>)
+        ensures b.valid()
+        ensures forall e1:T1 :: b.in1(e1) == false
+        ensures forall e2:T2 :: b.in2(e2) == false
+        ensures b.Keys() == {}
+        ensures b.Values() == {}
+        ensures b.Items() == {}
+    {
+        return BijectiveMap(map[], map[]);
     }
 }
